remove a few more int methods, get c++ backend working

lib/Base/total_order.i.dfy
@@ -712,18 +712,13 @@ module Integer_Order refines Total_Order {
 
   function SomeElement() : Element { 0 }
 
-  predicate method lte(a: Element, b: Element) {
+  predicate lte(a: Element, b: Element) {
     reveal_ltedef();
     ltedef(a, b)
   }
 
-  predicate method {:opaque} ltedef(a: Element, b: Element) {
+  predicate {:opaque} ltedef(a: Element, b: Element) {
     a <= b
-  }
-
-  method cmp(a: Element, b: Element) returns (c: int32)
-  {
-    return if a < b then -1 else if a > b then 1 else 0;
   }
 }
 
